some proof on compiling clightp

compcertox/ClightP.v
@@ -11,9 +11,9 @@ Require Import Ctypes Cop Clight.
 Module ClightP.
 
   Inductive val : Type :=
-  | Val : Values.val -> val
-  | Array : nat -> ZMap.t val -> val
-  | Struct : list ident -> PMap.t val -> val.
+  | Val : Values.val -> type -> val.
+  (* | Array : nat -> ZMap.t val -> val *)
+  (* | Struct : list ident -> PMap.t val -> val. *)
 
   Record privvar (V: Type) : Type :=
     mkprivvar {
@@ -37,8 +37,8 @@ Module ClightP.
   | Esizeof: type -> type -> expr         (**r size of a type *)
   | Ealignof: type -> type -> expr        (**r alignment of a type *)
   (* two new cases for persistent data and struct and array *)
-  | Epvar : ident -> type -> expr
-  | Eaccess : expr -> Z + ident -> type -> expr.
+  | Epvar : ident -> type -> expr.
+  (* | Eaccess : expr -> Z + ident -> type -> expr. *)
 
   Definition typeof (e: expr) : type :=
     match e with
@@ -57,7 +57,7 @@ Module ClightP.
     | Esizeof _ ty => ty
     | Ealignof _ ty => ty
     | Epvar _ ty => ty
-    | Eaccess _ _ ty => ty
+    (* | Eaccess _ _ ty => ty *)
     end.
 
   Inductive statement : Type :=
@@ -130,7 +130,6 @@ Module ClightP.
     | External id args res cc => Tfunction args res cc
     end.
 
-
   Record program : Type := {
       prog_defs: list (ident * globdef fundef type);
       prog_private: list (ident * privvar type);
@@ -193,58 +192,60 @@ Module ClightP.
       Variable pe: penv.
       Variable m: mem.
 
-      Coercion Val : Values.val >-> val.
+      (* Coercion Val : Values.val >-> val. *)
 
       Inductive eval_expr: expr -> val -> Prop :=
       | eval_Econst_int:   forall i ty,
-          eval_expr (Econst_int i ty) (Vint i)
+          eval_expr (Econst_int i ty) (Val (Vint i) ty)
       | eval_Econst_float:   forall f ty,
-          eval_expr (Econst_float f ty) (Vfloat f)
+          eval_expr (Econst_float f ty) (Val (Vfloat f) ty)
       | eval_Econst_single:   forall f ty,
-          eval_expr (Econst_single f ty) (Vsingle f)
+          eval_expr (Econst_single f ty) (Val (Vsingle f) ty)
       | eval_Econst_long:   forall i ty,
-          eval_expr (Econst_long i ty) (Vlong i)
+          eval_expr (Econst_long i ty) (Val (Vlong i) ty)
       | eval_Etempvar:  forall id ty v,
           le!id = Some v ->
-          eval_expr (Etempvar id ty) v
+          eval_expr (Etempvar id ty) (Val v ty)
       | eval_Eaddrof: forall a ty loc ofs,
           eval_lvalue a loc ofs Full ->
-          eval_expr (Eaddrof a ty) (Vptr loc ofs)
-      | eval_Eunop:  forall op a ty v1 v,
-          eval_expr a (Val v1) ->
+          eval_expr (Eaddrof a ty) (Val (Vptr loc ofs) ty)
+      | eval_Eunop:  forall op a ty v1 v tyv,
+          eval_expr a (Val v1 tyv) ->
           sem_unary_operation op v1 (typeof a) m = Some v ->
-          eval_expr (Eunop op a ty) v
-      | eval_Ebinop: forall op a1 a2 ty v1 v2 v,
-          eval_expr a1 (Val v1) ->
-          eval_expr a2 (Val v2) ->
+          eval_expr (Eunop op a ty) (Val v ty)
+      | eval_Ebinop: forall op a1 a2 ty v1 v2 v tyv1 tyv2,
+          eval_expr a1 (Val v1 tyv1) ->
+          eval_expr a2 (Val v2 tyv2) ->
           sem_binary_operation ge op v1 (typeof a1) v2 (typeof a2) m = Some v ->
-          eval_expr (Ebinop op a1 a2 ty) v
-      | eval_Ecast:   forall a ty v1 v,
-          eval_expr a (Val v1) ->
+          eval_expr (Ebinop op a1 a2 ty) (Val v ty)
+      | eval_Ecast:   forall a ty v1 v tyv,
+          eval_expr a (Val v1 tyv) ->
           sem_cast v1 (typeof a) ty m = Some v ->
-          eval_expr (Ecast a ty) v
+          eval_expr (Ecast a ty) (Val v ty)
       | eval_Esizeof: forall ty1 ty,
-          eval_expr (Esizeof ty1 ty) (Vptrofs (Ptrofs.repr (sizeof ge ty1)))
+          eval_expr (Esizeof ty1 ty) (Val (Vptrofs (Ptrofs.repr (sizeof ge ty1))) ty)
       | eval_Ealignof: forall ty1 ty,
-          eval_expr (Ealignof ty1 ty) (Vptrofs (Ptrofs.repr (alignof ge ty1)))
+          eval_expr (Ealignof ty1 ty) (Val (Vptrofs (Ptrofs.repr (alignof ge ty1))) ty)
       | eval_Elvalue: forall a loc ofs bf v,
           eval_lvalue a loc ofs bf ->
           deref_loc (typeof a) m loc ofs bf v ->
-          eval_expr a v
+          eval_expr a (Val v (typeof a))
       (* the new case *)
       | eval_Epvar: forall id ty v,
-          pe!id = Some v ->
-          eval_expr (Epvar id ty) v
-      | eval_Earray: forall a i ty v sz vs,
-          eval_expr a (Array sz vs) ->
-          i < Z.of_nat sz ->
-          ZMap.get i vs = v ->
-          eval_expr (Eaccess a (inl i) ty) v
-      | eval_Estruct: forall a f ty v fs vs,
-          eval_expr a (Struct fs vs) ->
-          In f fs ->
-          PMap.get f vs = v ->
-          eval_expr (Eaccess a (inr f) ty) v
+          (* note that we require the types of the value and the expression to
+             be the same *)
+          pe!id = Some (Val v ty) ->
+          eval_expr (Epvar id ty) (Val v ty)
+      (* | eval_Earray: forall a i ty v sz vs, *)
+      (*     eval_expr a (Array sz vs) -> *)
+      (*     i < Z.of_nat sz -> *)
+      (*     ZMap.get i vs = v -> *)
+      (*     eval_expr (Eaccess a (inl i) ty) v *)
+      (* | eval_Estruct: forall a f ty v fs vs, *)
+      (*     eval_expr a (Struct fs vs) -> *)
+      (*     In f fs -> *)
+      (*     PMap.get f vs = v -> *)
+      (*     eval_expr (Eaccess a (inr f) ty) v *)
 
       with eval_lvalue: expr -> block -> ptrofs -> bitfield -> Prop :=
       | eval_Evar_local:   forall id l ty,
@@ -254,17 +255,17 @@ Module ClightP.
           e!id = None ->
           Genv.find_symbol ge id = Some l ->
           eval_lvalue (Evar id ty) l Ptrofs.zero Full
-      | eval_Ederef: forall a ty l ofs,
-          eval_expr a (Vptr l ofs) ->
+      | eval_Ederef: forall a ty l ofs tya,
+          eval_expr a (Val (Vptr l ofs) tya) ->
           eval_lvalue (Ederef a ty) l ofs Full
-      | eval_Efield_struct:   forall a i ty l ofs id co att delta bf,
-          eval_expr a (Vptr l ofs) ->
+      | eval_Efield_struct:   forall a i ty l ofs id co att delta bf tya,
+          eval_expr a (Val (Vptr l ofs) tya) ->
           typeof a = Tstruct id att ->
           ge.(genv_cenv)!id = Some co ->
           field_offset ge i (co_members co) = OK (delta, bf) ->
           eval_lvalue (Efield a i ty) l (Ptrofs.add ofs (Ptrofs.repr delta)) bf
-      | eval_Efield_union:   forall a i ty l ofs id co att delta bf,
-          eval_expr a (Vptr l ofs) ->
+      | eval_Efield_union:   forall a i ty l ofs id co att delta bf tya,
+          eval_expr a (Val (Vptr l ofs) tya) ->
           typeof a = Tunion id att ->
           ge.(genv_cenv)!id = Some co ->
           union_field_offset ge i (co_members co) = OK (delta, bf) ->
@@ -277,8 +278,8 @@ Module ClightP.
       Inductive eval_exprlist: list expr -> typelist -> list Values.val -> Prop :=
       | eval_Enil:
         eval_exprlist nil Tnil nil
-      | eval_Econs:   forall a bl ty tyl v1 v2 vl,
-          eval_expr a (Val v1) ->
+      | eval_Econs:   forall a bl ty tyl v1 v2 vl tya,
+          eval_expr a (Val v1 tya) ->
           sem_cast v1 (typeof a) ty m = Some v2 ->
           eval_exprlist bl tyl vl ->
           eval_exprlist (a :: bl) (Tcons ty tyl) (v2 :: vl).
@@ -360,51 +361,52 @@ Module ClightP.
                end
            end.
 
-    Fixpoint update_penv_helper (a: expr) (v: val) (w: Values.val) : option (ident * val) :=
-      match a, v with
-      | Epvar i _, Val _ => Some (i, Val w)
-      | Eaccess e (inl x) _, Array sz vs =>
-          match update_penv_helper e (ZMap.get x vs) w with
-          | Some (i, v') => Some (i, Array sz (ZMap.set x v' vs))
-          | None => None
-          end
-      | Eaccess e (inr f) _, Struct fs vs =>
-          match update_penv_helper e (PMap.get f vs) w with
-          | Some (i, v') => Some (i, Struct fs (PMap.set f v' vs))
-          | None => None
-          end
-      | _, _ => None
-      end.
+    (* Fixpoint update_penv_helper (a: expr) (v: val) (w: Values.val) tyw : option (ident * val) := *)
+    (*   match a, v with *)
+    (*   | Epvar i _, Val _ _ => Some (i, Val w tyw) *)
+    (*   | Eaccess e (inl x) _, Array sz vs => *)
+    (*       match update_penv_helper e (ZMap.get x vs) w tyw with *)
+    (*       | Some (i, v') => Some (i, Array sz (ZMap.set x v' vs)) *)
+    (*       | None => None *)
+    (*       end *)
+    (*   | Eaccess e (inr f) _, Struct fs vs => *)
+    (*       match update_penv_helper e (PMap.get f vs) w tyw with *)
+    (*       | Some (i, v') => Some (i, Struct fs (PMap.set f v' vs)) *)
+    (*       | None => None *)
+    (*       end *)
+    (*   | _, _ => None *)
+    (*   end. *)
 
     Variable function_entry:
       function -> list Values.val -> mem -> env -> temp_env -> mem -> Prop.
 
     Inductive step: state * penv -> trace -> state * penv -> Prop :=
 
-    | step_assign:   forall f a1 a2 k e le pe m loc ofs bf v2 v m',
+    | step_assign:   forall f a1 a2 k e le pe m loc ofs bf v2 v m' tyv,
         eval_lvalue e le pe m a1 loc ofs bf ->
-        eval_expr e le pe m a2 (Val v2) ->
+        eval_expr e le pe m a2 (Val v2 tyv) ->
         sem_cast v2 (typeof a2) (typeof a1) m = Some v ->
         assign_loc ge (typeof a1) m loc ofs bf v m' ->
         step (State f (Sassign a1 a2) k e le m, pe)
              E0 (State f Sskip k e le m', pe)
 
-    | step_set:   forall f id a k e le pe m v,
-        eval_expr e le pe m a (Val v) ->
+    | step_set:   forall f id a k e le pe m v tyv,
+        eval_expr e le pe m a (Val v tyv) ->
         step (State f (Sset id a) k e le m, pe)
              E0 (State f Sskip k e (PTree.set id v le) m, pe)
+    (* we need a penv_loc and define something like assign_loc *)
+    (* By_value update *)
+    | step_update: forall f a2 k e le pe m id ty new_v old_v ch,
+        pe ! id = Some (Val old_v ty) ->
+        access_mode ty = By_value ch ->
+        eval_expr e le pe m a2 (Val new_v ty) ->
+        val_casted new_v ty ->
+        step (State f (Supdate (Epvar id ty) a2) k e le m, pe)
+             E0 (State f Sskip k e le m, PTree.set id (Val new_v ty) pe)
 
-    | step_update: forall f a1 a2 k e le pe m id v w v' w',
-        eval_expr e le pe m a1 v ->
-        eval_expr e le pe m a2 (Val w) ->
-        sem_cast w (typeof a2) (typeof a1) m = Some w' ->
-        update_penv_helper a1 v w = Some (id, v') ->
-        step (State f (Supdate a1 a2) k e le m, pe)
-             E0 (State f Sskip k e le m, PTree.set id v pe)
-
-    | step_call:   forall f optid a al k e le pe m tyargs tyres cconv vf vargs fd,
+    | step_call:   forall f optid a al k e le pe m tyargs tyres cconv vf vargs fd tyvf,
         classify_fun (typeof a) = fun_case_f tyargs tyres cconv ->
-        eval_expr e le pe m a (Val vf) ->
+        eval_expr e le pe m a (Val vf tyvf) ->
         eval_exprlist e le pe m al tyargs vargs ->
         Genv.find_funct ge vf = Some fd ->
         type_of_fundef fd = Tfunction tyargs tyres cconv ->
@@ -430,8 +432,8 @@ Module ClightP.
         step (State f Sbreak (Kseq s k) e le m, pe)
              E0 (State f Sbreak k e le m, pe)
 
-    | step_ifthenelse:  forall f a s1 s2 k e le pe m v1 b,
-        eval_expr e le pe m a (Val v1) ->
+    | step_ifthenelse:  forall f a s1 s2 k e le pe m v1 b tyv,
+        eval_expr e le pe m a (Val v1 tyv) ->
         bool_val v1 (typeof a) m = Some b ->
         step (State f (Sifthenelse a s1 s2) k e le m, pe)
              E0 (State f (if b then s1 else s2) k e le m, pe)
@@ -457,8 +459,8 @@ Module ClightP.
         Mem.free_list m (blocks_of_env e) = Some m' ->
         step (State f (Sreturn None) k e le m, pe)
              E0 (Returnstate Vundef (call_cont k) m', pe)
-    | step_return_1: forall f a k e le pe m v v' m',
-        eval_expr e le pe m a (Val v) ->
+    | step_return_1: forall f a k e le pe m v v' m' tyv,
+        eval_expr e le pe m a (Val v tyv) ->
         sem_cast v (typeof a) f.(fn_return) m = Some v' ->
         Mem.free_list m (blocks_of_env e) = Some m' ->
         step (State f (Sreturn (Some a)) k e le m, pe)
@@ -469,8 +471,8 @@ Module ClightP.
         step (State f Sskip k e le m, pe)
              E0 (Returnstate Vundef k m', pe)
 
-    | step_switch: forall f a sl k e le pe m v n,
-        eval_expr e le pe m a (Val v) ->
+    | step_switch: forall f a sl k e le pe m v n tyv,
+        eval_expr e le pe m a (Val v tyv) ->
         sem_switch_arg v (typeof a) = Some n ->
         step (State f (Sswitch a sl) k e le m, pe)
              E0 (State f (seq_of_labeled_statement (select_switch n sl)) (Kswitch k) e le m, pe)
@@ -517,20 +519,20 @@ Module ClightP.
           (cq vf (signature_of_type targs tres tcc) vargs m, pe)
           (Callstate vf vargs Kstop m, pe).
 
-    Inductive at_external: state * penv -> c_query * penv -> Prop :=
+    Inductive at_external: state * penv -> c_query -> Prop :=
     | at_external_intro name sg targs tres cconv vf vargs k m pe:
       let f := External (EF_external name sg) targs tres cconv in
       Genv.find_funct ge vf = Some f ->
       at_external
         (Callstate vf vargs k m, pe)
-        (cq vf sg vargs m, pe).
+        (cq vf sg vargs m).
 
-    Inductive after_external: state * penv -> c_reply * penv -> state * penv -> Prop :=
-    | after_external_intro vf vargs k m pe vres m' pe':
+    Inductive after_external: state * penv -> c_reply -> state * penv -> Prop :=
+    | after_external_intro vf vargs k m pe vres m':
       after_external
         (Callstate vf vargs k m, pe)
-        (cr vres m', pe')
-        (Returnstate vres k m', pe').
+        (cr vres m')
+        (Returnstate vres k m', pe).
 
     Inductive final_state: state * penv -> c_reply * penv -> Prop :=
     | final_state_intro: forall r m pe,
@@ -573,29 +575,21 @@ Module ClightP.
   Definition add_privates (pe: penv) (x: list (ident * privvar type)) : penv :=
     List.fold_left add_private x pe.
 
-  Program Definition clightp1 (p : program) : esemantics li_c li_c :=
-    {|
-      pstate := penv;
-      init_pstate := add_privates empty_penv (prog_private p);
-      esem := Semantics_gen step1
-                            initial_state
-                            at_external
-                            (fun _ => after_external)
-                            (fun _ => final_state)
-                            globalenv p;
-    |}.
+  Program Definition clightp1 (p : program) : semantics _ (li_c@penv) :=
+      Semantics_gen step1
+        initial_state
+        at_external
+        (fun _ => after_external)
+        (fun _ => final_state)
+        globalenv p.
 
-  Program Definition clightp2 (p : program) : esemantics li_c li_c :=
-    {|
-      pstate := penv;
-      init_pstate := add_privates empty_penv (prog_private p);
-      esem := Semantics_gen step2
-                            initial_state
-                            at_external
-                            (fun _ => after_external)
-                            (fun _ => final_state)
-                            globalenv p;
-    |}.
+  Program Definition clightp2 (p : program) : semantics _ (li_c@penv) :=
+      Semantics_gen step2
+        initial_state
+        at_external
+        (fun _ => after_external)
+        (fun _ => final_state)
+        globalenv p.
 
 End ClightP.
 
@@ -609,14 +603,14 @@ Section TRANSF.
   Fixpoint transl_lvalue (a: expr) : res Clight.expr :=
     match a with
     | Epvar i ty => OK (Clight.Evar i ty)
-    | Eaccess e (inr f) ty =>
-        do te <- transl_lvalue e;
-        OK (Clight.Efield te f ty)
-    | Eaccess e (inl i) ty =>
-        do te <- transl_lvalue e;
-        OK (Clight.Ebinop Oadd te
-                             (Clight.Econst_int (Int.repr i) (Tint I32 Unsigned noattr))
-                             (Tpointer ty noattr))
+    (* | Eaccess e (inr f) ty => *)
+    (*     do te <- transl_lvalue e; *)
+    (*     OK (Clight.Efield te f ty) *)
+    (* | Eaccess e (inl i) ty => *)
+    (*     do te <- transl_lvalue e; *)
+    (*     OK (Clight.Ebinop Oadd te *)
+    (*                          (Clight.Econst_int (Int.repr i) (Tint I32 Unsigned noattr)) *)
+    (*                          (Tpointer ty noattr)) *)
     | _ => Error (msg "transl_lvalue")
     end.
 
@@ -634,13 +628,13 @@ Section TRANSF.
     | Eaddrof e ty =>
         do te <- transl_expr e;
         OK (Clight.Eaddrof te ty)
-    | Eunop o e ty =>
+    | Eunop op e ty =>
         do te <- transl_expr e;
-        OK (Clight.Eunop o te ty)
-    | Ebinop o e1 e2 ty =>
+        OK (Clight.Eunop op te ty)
+    | Ebinop op e1 e2 ty =>
         do te1 <- transl_expr e1;
         do te2 <- transl_expr e2;
-        OK (Clight.Ebinop o te1 te2 ty)
+        OK (Clight.Ebinop op te1 te2 ty)
     | Ecast e ty =>
         do te <- transl_expr e;
         OK (Clight.Ecast te ty)
@@ -650,20 +644,28 @@ Section TRANSF.
     | Esizeof t ty => OK (Clight.Esizeof t ty)
     | Ealignof t ty => OK (Clight.Ealignof t ty)
     | Epvar i ty =>
-        OK (Clight.Ederef (Clight.Evar i ty) ty)
-    | Eaccess e (inr f) ty =>
-        do te <- transl_lvalue e;
-        OK (Clight.Ederef (Clight.Efield te f ty) ty)
-    | Eaccess e (inl i) ty =>
-        do te <- transl_lvalue e;
-        OK (Clight.Ederef
-              (Clight.Ebinop Oadd te
-                             (Clight.Econst_int (Int.repr i) (Tint I32 Unsigned noattr))
-                             (Tpointer ty noattr)) ty)
+        OK (Clight.Evar i ty)
+    (* | Eaccess e (inr f) ty => *)
+    (*     do te <- transl_lvalue e; *)
+    (*     OK (Clight.Ederef (Clight.Efield te f ty) ty) *)
+    (* | Eaccess e (inl i) ty => *)
+    (*     do te <- transl_lvalue e; *)
+    (*     OK (Clight.Ederef *)
+    (*           (Clight.Ebinop Oadd te *)
+    (*                          (Clight.Econst_int (Int.repr i) (Tint I32 Unsigned noattr)) *)
+    (*                          (Tpointer ty noattr)) ty) *)
     end.
 
-  Fixpoint transl_arglist (xs: list expr): res (list Clight.expr).
-  Admitted.
+  Fixpoint transl_exprlist (xs: list expr): res (list Clight.expr) :=
+    match xs with
+    | nil => OK nil
+    | e :: es =>
+        do te <- transl_expr e;
+        do tes <- transl_exprlist es;
+        OK (te :: tes)
+    end.
+
+  Definition transl_arglist := transl_exprlist.
 
   Fixpoint transl_statement (s: statement) : res Clight.statement :=
     match s with
@@ -744,8 +746,7 @@ Section TRANSF.
 
   Definition transl_globvar (id: ident) (ty: type) := OK ty.
 
-  Definition val_init_data (v: val) : res (list init_data).
-  Admitted.
+  Definition val_init_data (v: val) : res (list init_data). Admitted.
 
   Definition transl_privvar {V} (v: privvar V) :=
     do x <- val_init_data (pvar_init _ v);
@@ -778,6 +779,1147 @@ Section TRANSF.
 
 End TRANSF.
 
+Require Import LogicalRelations.
+Require Import OptionRel.
+Require Import Lia.
+
+Open Scope Z_scope.
+
+Section MEM_SAME_EXCEPT.
+
+  Variable (P: block -> Z -> Prop).
+  Hypothesis P_dec: forall b ofs, {P b ofs} + {~ P b ofs}.
+
+  Record mem_same_except  (m1: Mem.mem) (m2: Mem.mem) :=
+    {
+      same_support: Mem.support m1 = Mem.support m2;
+      same_perm: forall b ofs k p, ~ P b ofs -> Mem.perm m1 b ofs k p <-> Mem.perm m2 b ofs k p;
+      same_content: forall b ofs, ~ P b ofs -> ZMap.get ofs (NMap.get _ b (Mem.mem_contents m1))
+                                         = ZMap.get ofs (NMap.get _ b (Mem.mem_contents m2));
+      diff_perm: forall b ofs, P b ofs -> loc_out_of_bounds m1 b ofs;
+    }.
+
+  Instance valid_pointer_mse:
+    Monotonic
+      (@Mem.valid_pointer)
+      (mem_same_except ++> - ==> - ==> leb).
+  Proof.
+    do 4 rstep. destruct Mem.valid_pointer eqn: X; try easy.
+    cbn. rewrite !Mem.valid_pointer_nonempty_perm in *.
+    edestruct P_dec.
+    - eapply diff_perm in p; eauto. exfalso. apply p.
+      eapply Mem.perm_max; eauto.
+    - rewrite <- same_perm; eauto.
+  Qed.
+
+  Instance weak_valid_pointer_mse:
+    Monotonic
+      (@Mem.weak_valid_pointer)
+      (mem_same_except ++> - ==> - ==> leb).
+  Proof.
+    unfold Mem.weak_valid_pointer. do 4 rstep.
+    destruct orb eqn: X.
+    - simpl. rewrite orb_true_iff in *.
+      destruct X; [ left | right ]; apply valid_pointer_mse in H.
+      specialize (H x0 x1). rewrite H0 in H. eauto.
+      specialize (H x0 (x1 - 1)%Z). rewrite H0 in H. eauto.
+    - easy.
+  Qed.
+
+  Instance bool_val_mse:
+    Monotonic
+      (@bool_val)
+      (- ==> - ==> mem_same_except ++> option_le eq).
+  Proof. unfold bool_val. rauto. Qed.
+
+  Instance sem_unary_operation_mse:
+    Monotonic
+      (@sem_unary_operation)
+      (- ==> - ==> - ==> mem_same_except ++> option_le eq).
+  Proof.
+    unfold sem_unary_operation.
+    unfold sem_notbool, sem_notint, sem_neg, sem_absfloat.
+    repeat rstep. f_equal. congruence.
+  Qed.
+
+  Instance sem_cast_mse:
+    Monotonic
+      (@Cop.sem_cast)
+      (- ==> - ==> - ==> mem_same_except ++> option_le eq).
+  Proof. unfold Cop.sem_cast. repeat rstep. Qed.
+
+  Instance sem_binarith_mse:
+    Monotonic
+      (@Cop.sem_binarith)
+      (- ==> - ==> - ==> - ==> - ==> - ==> - ==> - ==> mem_same_except ++> option_le eq).
+  Proof. unfold Cop.sem_binarith. repeat rstep. Qed.
+
+  Instance cmp_ptr_mse:
+    Related
+      (@Cop.cmp_ptr)
+      (@Cop.cmp_ptr)
+      (mem_same_except ++> - ==> - ==> - ==> option_le eq).
+  Proof.
+    rstep. rstep. rstep. rstep. rstep.
+    unfold Cop.cmp_ptr. rstep. rstep. rewrite H0. reflexivity. rstep.
+    - rstep. unfold Val.cmplu_bool. repeat rstep.
+    - rstep. unfold Val.cmpu_bool. repeat rstep.
+      Unshelve. all: eauto.
+  Qed.
+
+  Instance sem_cmp_mse:
+    Monotonic
+      (@Cop.sem_cmp)
+      (- ==> - ==> - ==> - ==> - ==> mem_same_except ++> option_le eq).
+  Proof. unfold Cop.sem_cmp. repeat rstep. Qed.
+
+  Instance sem_binary_operation_mse:
+    Monotonic
+      (@sem_binary_operation)
+      (- ==> - ==> - ==> - ==> - ==> - ==> mem_same_except ++> option_le eq).
+  Proof.
+    unfold sem_binary_operation.
+    unfold
+      Cop.sem_add,
+      Cop.sem_add_ptr_int,
+      Cop.sem_add_ptr_long,
+      Cop.sem_sub,
+      Cop.sem_mul,
+      Cop.sem_div,
+      Cop.sem_mod,
+      Cop.sem_and,
+      Cop.sem_or,
+      Cop.sem_xor,
+      Cop.sem_shl,
+      Cop.sem_shr.
+    repeat rstep.
+  Qed.
+
+(*     Lemma bool_val_inject: *)
+(*   forall f m m' v ty b tv, *)
+(*   bool_val v ty m = Some b -> *)
+(*   Val.inject f v tv -> *)
+(*   Mem.inject f m m' -> *)
+(*   bool_val tv ty m' = Some b. *)
+(* Proof. *)
+(*   intros. eapply bool_val_inj; eauto. *)
+(*   intros; eapply Mem.weak_valid_pointer_inject_val; eauto. *)
+(* Qed. *)
+
+  (* Lemma P_range_dec : forall (b : block) (lo hi : Z), *)
+  (*     {forall ofs, (lo <= ofs < hi)%Z -> P b ofs} + {~ (forall ofs, (lo <= ofs < hi)%Z -> P b ofs)}. *)
+  (* Admitted. *)
+
+  Lemma perm_mse m1 m2 b ofs k p:
+    mem_same_except m1 m2 ->
+    Mem.perm m1 b ofs k p ->
+    Mem.perm m2 b ofs k p.
+  Proof.
+    intros HM H.
+    destruct (P_dec b ofs) as [X|X].
+    - eapply diff_perm in X; eauto.
+      exfalso. eauto with mem.
+    - rewrite <- same_perm; eauto.
+  Qed.
+
+  Lemma range_perm_mse m1 m2 b lo hi k p:
+    mem_same_except m1 m2 ->
+    Mem.range_perm m1 b lo hi k p ->
+    Mem.range_perm m2 b lo hi k p.
+  Proof.
+    intros HM H ofs X. specialize (H _ X).
+    eauto using perm_mse.
+  Qed.
+
+  Instance load_mse:
+    Monotonic
+      (@Mem.load)
+      (- ==> mem_same_except ++> - ==> - ==> option_le eq).
+  Proof.
+    repeat rstep. destruct Mem.load eqn: X; try constructor.
+    rename x1 into b. rename x2 into ofs. rename x into ch.
+    rename x0 into m1. rename y into m2.
+    exploit Mem.load_valid_access. eauto. intros [A B].
+    exploit Mem.valid_access_load. split. eapply range_perm_mse; eauto. apply B.
+    intros [w Y]. rewrite Y. constructor.
+    exploit Mem.load_result. apply X.
+    exploit Mem.load_result. apply Y. intros -> ->.
+    f_equal. apply Mem.getN_exten.
+    intros i Hi. apply same_content; eauto.
+    intros contra. eapply diff_perm in contra; eauto.
+    apply contra. rewrite <- size_chunk_conv in Hi.
+    specialize (A _ Hi). eauto with mem.
+  Qed.
+
+  Instance loadv_mse:
+    Monotonic
+      (@Mem.loadv)
+      (- ==> mem_same_except ++> - ==> option_le eq).
+  Proof. unfold Mem.loadv. repeat rstep. Qed.
+
+  Instance load_bitfield_mse:
+    Monotonic
+      (@load_bitfield)
+      (- ==> - ==> - ==> - ==> - ==> mem_same_except ++> - ==> - ==> impl).
+  Proof.
+    repeat rstep. intros Hv.
+    destruct Hv as [sz sg1 attr sg pos width m v' ? Hpos Hwidth Hpw Hsg1 Hload].
+    transport Hload. subst.
+    constructor; eauto.
+  Qed.
+
+  Instance deref_loc_mse a:
+    Monotonic
+      (@deref_loc a)
+      (mem_same_except ++> - ==> - ==> - ==> - ==> impl).
+  Proof.
+    repeat rstep. intros A. inv A; eauto using @deref_loc_reference, @deref_loc_copy.
+    - transport H1. subst. eapply deref_loc_value; eauto.
+    - eapply deref_loc_bitfield. eapply load_bitfield_mse; eauto.
+  Qed.
+
+  Lemma get_setN_inside:
+    forall vl p q c,
+      p <= q < p + Z.of_nat (length vl) ->
+      (ZMap.get q (Mem.setN vl p c)) = nth (Z.to_nat (q - p)) vl Undef.
+  Proof.
+    induction vl; intros.
+    simpl in H. extlia.
+    simpl length in H. rewrite Nat2Z.inj_succ in H. simpl.
+    destruct (zeq p q).
+    - subst q. rewrite Mem.setN_outside by lia. rewrite ZMap.gss.
+      replace (p - p) with 0 by lia. reflexivity.
+    - rewrite IHvl by lia. destruct H as [A B].
+      replace (q - p) with (Z.succ (q - p - 1)) by lia.
+      rewrite Z2Nat.inj_succ. 2: lia.
+      f_equal. f_equal. lia.
+  Qed.
+
+  Instance store_mse:
+    Monotonic
+      (@Mem.store)
+      (- ==> mem_same_except ++> - ==> - ==> - ==> option_le mem_same_except).
+  Proof.
+    repeat rstep. destruct Mem.store eqn: X; try constructor.
+    rename x into ch. rename x1 into b. rename x2 into ofs. rename x3 into v.
+    rename x0 into m1. rename y into m2.
+    exploit Mem.store_valid_access_3; eauto. intros [A B].
+    edestruct Mem.valid_access_store as [n Y]. split. 2: eauto.
+    eapply range_perm_mse; eauto.
+    rewrite Y. constructor.
+    constructor.
+    - exploit Mem.support_store. apply X. intros ->.
+      exploit Mem.support_store. apply Y. intros ->.
+      apply H.
+    - intros bx ofsx k p HP. split; intros.
+      + eapply Mem.perm_store_1; eauto.
+        rewrite <- same_perm. 2-3: eauto.
+        eapply Mem.perm_store_2; eauto.
+      + eapply Mem.perm_store_1; eauto.
+        rewrite same_perm. 2-3: eauto.
+        eapply Mem.perm_store_2; eauto.
+    - intros bx ofsx HP.
+      exploit Mem.store_mem_contents. apply X. intros ->.
+      exploit Mem.store_mem_contents. apply Y. intros ->.
+      exploit same_content; eauto. intros C.
+      rewrite !NMap.gsspec.
+      destruct (NMap.elt_eq bx b).
+      + subst. destruct (zlt ofsx ofs).
+        * now rewrite !Mem.setN_outside by lia.
+        * destruct (zle (ofs + Z.of_nat (length (encode_val ch v))) ofsx).
+          now rewrite !Mem.setN_outside by lia.
+          now rewrite !get_setN_inside by lia.
+      + apply C.
+    - intros bx ofsx HP C.
+      eapply diff_perm; eauto. eauto with mem.
+  Qed.
+
+  Transparent Mem.loadbytes Mem.storebytes.
+  Instance storev_mse:
+    Monotonic
+      (@Mem.storev)
+      (- ==> mem_same_except ++> - ==> - ==> option_le mem_same_except).
+  Proof. unfold Mem.storev. repeat rstep. Qed.
+
+  Instance loadbytes_mse:
+    Monotonic
+      (@Mem.loadbytes)
+      (mem_same_except ++> - ==> - ==> - ==> option_le eq).
+  Proof.
+    repeat rstep. destruct Mem.loadbytes eqn: X; try constructor.
+    unfold Mem.loadbytes in *.
+    rename x0 into b. rename x1 into ofs. rename x2 into sz.
+    rename x into m1. rename y into m2.
+    destruct (Mem.range_perm_dec m1 b ofs (ofs + sz) Cur Readable); inv X.
+    destruct Mem.range_perm_dec.
+    - constructor. apply Mem.getN_exten. intros i Hi.
+      apply same_content; eauto. intros HP.
+      eapply diff_perm; eauto.
+      destruct (zle 0 sz); eauto.
+      + rewrite Z2Nat.id in Hi by lia. eauto with mem.
+      + rewrite Z_to_nat_neg in Hi by lia. lia.
+    - exfalso. apply n.
+      eapply range_perm_mse; eauto.
+  Qed.
+
+  Instance storebytes_mse:
+    Monotonic
+      (@Mem.storebytes)
+      (mem_same_except ++> - ==> - ==> - ==> option_le mem_same_except).
+  Proof.
+    repeat rstep. destruct Mem.storebytes eqn: X; try constructor.
+    unfold Mem.storebytes in *.
+    rename x0 into b. rename x1 into ofs. rename x2 into vl.
+    rename x into m1. rename y into m2.
+    destruct (Mem.range_perm_dec m1 b ofs (ofs + Z.of_nat (Datatypes.length vl)) Cur Writable); inv X.
+    destruct Mem.range_perm_dec.
+    - constructor. constructor; cbn -[NMap.get].
+      + apply same_support; eauto.
+      + intros bx ofsx k p HP.
+        unfold Mem.perm. cbn.
+        apply same_perm; eauto.
+      + intros bx ofsx HP.
+        exploit same_content; eauto. intros A.
+        rewrite !NMap.gsspec.
+        destruct (NMap.elt_eq bx b).
+        * subst. destruct (zlt ofsx ofs).
+          -- now rewrite !Mem.setN_outside by lia.
+          -- destruct (zle (ofs + Z.of_nat (length vl)) ofsx).
+             now rewrite !Mem.setN_outside by lia.
+             now rewrite !get_setN_inside by lia.
+        * apply A.
+      + intros bx ofsx HP C.
+        eapply diff_perm; eauto.
+    - exfalso. apply n.
+      eauto using range_perm_mse.
+  Qed.
+  Opaque Mem.loadbytes Mem.storebytes.
+
+  Instance store_bitfield_mse:
+    Monotonic
+      (@store_bitfield)
+      (- ==> - ==> - ==> - ==> - ==> mem_same_except ++> - ==> - ==> % set_le (mem_same_except * eq)).
+  Proof.
+    repeat rstep.
+    intros [v m] Hv.
+    destruct Hv as [sz sg1 attr sg pos width m addr v n m' Hpos Hw Hpw Hsg1 Hload Hstore].
+    transport Hload. subst.
+    transport Hstore.
+    eexists (_, _). cbn. split; [ | rauto].
+    econstructor; eauto.
+  Qed.
+
+  Instance assign_loc_mse:
+    Monotonic
+      (@assign_loc)
+      (- ==> - ==> mem_same_except ++> - ==> - ==> - ==> - ==> set_le mem_same_except).
+  Proof.
+    repeat rstep. intros m A. inv A.
+    - transport H1. eexists; split; eauto.
+      eapply assign_loc_value; eauto.
+    - transport H4. subst.
+      transport H5.
+      eexists; split; eauto.
+      eapply assign_loc_copy; eauto.
+    - exploit store_bitfield_mse; eauto.
+      unfold uncurry. instantiate (8 := (_, _)). cbn. apply H0.
+      intros ([a b] & A & B). cbn in *. split_hyps. subst.
+      eexists. split; eauto.
+      eapply assign_loc_bitfield; eauto.
+  Qed.
+
+  Lemma mse_preserve mx m m' ch b ofs v:
+    mem_same_except mx m ->
+    Mem.store ch m b ofs v = Some m' ->
+    (forall i, ofs <= i < ofs + size_chunk ch -> P b i) ->
+    mem_same_except mx m'.
+  Proof.
+    intros H HST HX.
+    constructor.
+    - eapply Mem.support_store in HST.
+      rewrite HST. apply H.
+    - intros bx ofsx k p HP. split; intros.
+      + eapply Mem.perm_store_1; eauto.
+        rewrite <- same_perm; eauto.
+      + rewrite same_perm. 2-3: eauto.
+        eapply Mem.perm_store_2; eauto.
+    - intros bx ofsx HP.
+      erewrite same_content. 2-3: eauto.
+      exploit Mem.store_mem_contents; eauto. intros ->.
+      rewrite NMap.gsspec.
+      destruct (NMap.elt_eq bx b).
+      + subst. destruct (zlt ofsx ofs).
+        * now rewrite !Mem.setN_outside by lia.
+        * destruct (zle (ofs + Z.of_nat (length (encode_val ch v))) ofsx).
+          -- now rewrite !Mem.setN_outside by lia.
+          -- exfalso.
+             apply HP. apply HX.
+             rewrite encode_val_length in *.
+             unfold size_chunk_nat in *.
+             rewrite Z2Nat.id in *. lia.
+             destruct ch; cbn; lia.
+      + reflexivity.
+    - intros bx ofsx HP C.
+      eapply diff_perm; eauto.
+  Qed.
+
+End MEM_SAME_EXCEPT.
+
+(* Lemma transport_in_goal_manual `{Transport}: *)
+(*   forall (Q: Prop), (R a b) -> (PB -> Q) -> (PA -> Q). *)
+(* Proof. firstorder. Qed. *)
+
+(* Ltac transp H := *)
+(*   revert H; *)
+(*   lazymatch goal with *)
+(*   | |- ?PA -> ?Q => *)
+(*       eapply (transport_in_goal_manual (PA:=PA) Q) *)
+(*   end; *)
+(*   try solve [ rauto | rstep; eauto ]; intro H. *)
+
+Require Import AbRel.
+
+Fixpoint psizeof_ty (t: type) : Z :=
+  match t with
+  | Tvoid => 1
+  | Tint I8 _ _ => 1
+  | Tint I16 _ _ => 2
+  | Tint I32 _ _ => 4
+  | Tint IBool _ _ => 1
+  | Tlong _ _ => 8
+  | Tfloat F32 _ => 4
+  | Tfloat F64 _ => 8
+  | Tpointer _ _ => if Archi.ptr64 then 8 else 4
+  | _ => 0
+  end.
+
+Fixpoint psizeof (x: ClightP.val) : Z :=
+  match x with
+  | ClightP.Val _ ty => psizeof_ty ty
+  end.
+
+Definition penv_footprint (pe: ClightP.penv): list (ident * Z) :=
+  map (fun '(id, v) => (id, psizeof v)) (PTree.elements pe).
+
+(* Fixpoint pfield_offset_rec (s: PMap.t ClightP.val) (id: ident) (ms: list ident) (pos: Z) *)
+(*   {struct ms} : option Z := *)
+(*   match ms with *)
+(*   | nil => None *)
+(*   | m :: ms => *)
+(*       if ident_eq id m then Some pos *)
+(*       else *)
+(*         let x := PMap.get id s in *)
+(*         pfield_offset_rec s id ms (pos + psizeof x) *)
+(*   end. *)
+
+(* Definition pfield_offset (s: PMap.t ClightP.val) (id: ident) (ms: list ident) := *)
+(*   pfield_offset_rec s id ms 0. *)
+
+Inductive pvalue_match: block -> Z -> ClightP.val -> Mem.mem -> Prop :=
+| pval_match b ofs ty chunk v m:
+  access_mode ty = By_value chunk ->
+  Mem.load chunk m  b ofs = Some v ->
+  Mem.valid_access m chunk b ofs Writable ->
+  pvalue_match b ofs (ClightP.Val v ty) m.
+(* | parr_match b ofs n a m: *)
+(*   (forall i, i < n -> *)
+(*         let z := Z.of_nat i in *)
+(*         pvalue_match b (Ptrofs.add ofs (Ptrofs.repr z)) (ZMap.get z a) m) -> *)
+(*   pvalue_match b ofs (ClightP.Array n a) m *)
+(* | pstr_match b ofs l s m: *)
+(*   (forall p x, In p l -> pfield_offset s p l = Some x -> *)
+(*           pvalue_match b (Ptrofs.add ofs (Ptrofs.repr x)) (PMap.get p s) m) -> *)
+(*   pvalue_match b ofs (ClightP.Struct l s) m. *)
+
+Inductive penv_match: Genv.symtbl -> (ClightP.penv * Mem.mem) -> Mem.mem -> Prop :=
+| penv_match_intro se pe m tm
+    (MSAME: mem_same_except (locsp se (penv_footprint pe)) m tm)
+    (MDIFF: forall id v, PTree.get id pe = Some v ->
+                    exists b, Genv.find_symbol se id = Some b /\
+                           pvalue_match b 0 v tm)
+  : penv_match se (pe, m) tm.
+
+Inductive pmatch_query: Genv.symtbl -> query (li_c @ ClightP.penv) -> query li_c -> Prop :=
+| pmatch_query_intro se vf sg vargs m tm pe
+    (PM: penv_match se (pe, m) tm):
+  pmatch_query se (cq vf sg vargs m, pe) (cq vf sg vargs tm).
+
+Inductive pmatch_reply: Genv.symtbl -> reply (li_c @ ClightP.penv) -> reply li_c -> Prop :=
+| pmatch_reply_intro se rv m tm pe
+    (PM: penv_match se (pe, m) tm):
+  pmatch_reply se (cr rv m, pe) (cr rv tm).
+
+Program Definition cc_penv: callconv (li_c @ ClightP.penv) li_c :=
+  {|
+    (* the world is defined as the target program symbol table, which is
+       supposed to contain the variables in penv *)
+    ccworld := Genv.symtbl;
+    match_senv se se1 se2 := se = se1 /\ se = se2;
+    match_query := pmatch_query;
+    match_reply := pmatch_reply;
+  |}.
+Next Obligation. reflexivity. Qed.
+Next Obligation. inv H0. reflexivity. Qed.
+Next Obligation. inv H. reflexivity. Qed.
+
+Definition value_of (pv: ClightP.val) :=
+  match pv with
+  | ClightP.Val v _ => v
+  end.
+Definition type_of (pv: ClightP.val) :=
+  match pv with
+  | ClightP.Val _ ty => ty
+  end.
+
+Lemma size_type_chunk ty ch:
+  access_mode ty = By_value ch ->
+  size_chunk ch = psizeof_ty ty.
+Proof.
+  intros. destruct ty; inv H; cbn in *; try easy.
+  - destruct i; destruct s; inv H1; easy.
+  - destruct f; inv H1; easy.
+Qed.
+
+Lemma unchanged_on_pvalue_match P b ofs v m m':
+  pvalue_match b ofs v m -> Mem.unchanged_on P m m' ->
+  (forall i, ofs <= i < ofs + psizeof_ty (type_of v) -> P b i) ->
+  pvalue_match b ofs v m'.
+Proof.
+  intros A B C. inv A. econstructor; eauto.
+  unfold Mem.loadv in *.
+  eapply Mem.load_unchanged_on; eauto.
+  intros i Hi.
+  apply C. cbn. erewrite <- size_type_chunk; eauto.
+  destruct H1 as [D E]. split; eauto.
+  intros x Hx. specialize (D _ Hx).
+  eapply Mem.perm_unchanged_on; eauto.
+  apply C. cbn. erewrite <- size_type_chunk; eauto.
+Qed.
+
+Lemma eval_expr_type_same ge e le pe t x v:
+  ClightP.eval_expr ge e le pe t x v ->
+  type_of v = ClightP.typeof x.
+Admitted.
+
+Section PRESERVATION.
+
+  Definition ptree_disjoint {A B} (m: PTree.t A) (n: PTree.t B) :=
+    forall i v w, m ! i = Some v -> n ! i = Some w -> False.
+
+  Variable prog: ClightP.program.
+  Variable tprog: Clight.program.
+  Hypothesis TRANSL: transl_program prog = OK tprog.
+  (* match_senv is defined as equal. For now, we require the source and target
+     symbol tables to be the same and both carry the module static variables *)
+  Variable se: Genv.symtbl.
+  Let ge : ClightP.genv := ClightP.globalenv se prog.
+  Let tge : Clight.genv := Clight.globalenv se tprog.
+
+  Inductive pmatch_cont: (ClightP.cont * ClightP.penv) -> Clight.cont -> Prop :=
+  | pmatch_Kstop: forall pe, pmatch_cont (ClightP.Kstop, pe) Clight.Kstop
+  | pmatch_Kseq: forall s t k tk pe,
+      transl_statement s = OK t ->
+      pmatch_cont (k, pe) tk ->
+      pmatch_cont (ClightP.Kseq s k, pe) (Clight.Kseq t tk)
+  | pmatch_Kloop1: forall s1 s2 ts1 ts2 k tk pe,
+      transl_statement s1 = OK ts1 ->
+      transl_statement s2 = OK ts2 ->
+      pmatch_cont (k, pe) tk ->
+      pmatch_cont (ClightP.Kloop1 s1 s2 k, pe) (Clight.Kloop1 ts1 ts2 tk)
+  | pmatch_Kloop2: forall s1 s2 ts1 ts2 k tk pe,
+      transl_statement s1 = OK ts1 ->
+      transl_statement s2 = OK ts2 ->
+      pmatch_cont (k, pe) tk ->
+      pmatch_cont (ClightP.Kloop2 s1 s2 k, pe) (Clight.Kloop2 ts1 ts2 tk)
+  | pmatch_Kswitch: forall k tk pe,
+      pmatch_cont (k, pe) tk -> pmatch_cont (ClightP.Kswitch k, pe) (Clight.Kswitch tk)
+  | pmatch_Kcall: forall fid f tf e le k tk pe,
+      transl_function f = OK tf ->
+      pmatch_cont (k, pe) tk ->
+      ptree_disjoint e pe ->
+      pmatch_cont (ClightP.Kcall fid f e le k, pe) (Clight.Kcall fid tf e le tk).
+
+  Inductive pmatch_state: Genv.symtbl -> ClightP.state * ClightP.penv -> Clight.state -> Prop :=
+  | pmatch_State: forall se fs ss ks e le ms pe ft st kt mt
+      (TRF: transl_function fs = OK ft)
+      (TRS: transl_statement ss = OK st)
+      (MK: pmatch_cont (ks, pe) kt)
+      (MP: penv_match se (pe, ms) mt)
+      (DISJ: ptree_disjoint e pe),
+      pmatch_state se (ClightP.State fs ss ks e le ms, pe) (Clight.State ft st kt e le mt)
+  | pmatch_Callstate: forall se vf args ks kt ms mt pe
+      (MK: pmatch_cont (ks, pe) kt)
+      (MP: penv_match se (pe, ms) mt),
+      pmatch_state se (ClightP.Callstate vf args ks ms, pe) (Clight.Callstate vf args kt mt)
+  | pmatch_Returnstate: forall se rv ks kt ms mt pe
+      (MK: pmatch_cont (ks, pe) kt)
+      (MP: penv_match se (pe, ms) mt),
+      pmatch_state se (ClightP.Returnstate rv ks ms, pe) (Clight.Returnstate rv kt mt).
+
+  Definition transl_expr_typeof e te:
+    transl_expr e = OK te -> ClightP.typeof e = typeof te.
+  Proof.
+    intros TE; destruct e; monadInv TE; cbn in *; eauto.
+  Qed.
+
+  Lemma penv_footprint_dec:
+    forall pe b ofs, {locsp se (penv_footprint pe) b ofs} + {~ locsp se (penv_footprint pe) b ofs}.
+  Proof.
+    intros.
+  Admitted.
+
+  Lemma eval_expr_lvalue_correct :
+    forall e le m tm pe,
+      ptree_disjoint e pe ->
+      penv_match se (pe, m) tm ->
+      (forall expr v,
+          ClightP.eval_expr ge e le pe m expr v ->
+          forall texpr (TR: transl_expr expr = OK texpr),
+            Clight.eval_expr tge e le tm texpr (value_of v))
+      /\
+      (forall expr b ofs bf,
+         ClightP.eval_lvalue ge e le pe m expr b ofs bf ->
+         forall texpr (TR: transl_expr expr = OK texpr),
+           Clight.eval_lvalue tge e le tm texpr b ofs bf).
+  Proof.
+    intros e le t tm pe HE HP.
+    apply ClightP.eval_expr_lvalue_ind.
+    - intros. monadInv TR. constructor.
+    - intros. monadInv TR. constructor.
+    - intros. monadInv TR. constructor.
+    - intros. monadInv TR. constructor.
+    - intros. monadInv TR. constructor. eauto.
+    - intros. monadInv TR.
+      constructor. apply H0. apply EQ.
+    - intros. monadInv TR. econstructor; eauto.
+      erewrite <- transl_expr_typeof; eauto. inv HP.
+      pose proof (sem_unary_operation_mse _ (penv_footprint_dec pe)).
+      transport H1. subst. eauto.
+    - intros. monadInv TR. econstructor; eauto.
+      erewrite <- !transl_expr_typeof; eauto. inv HP.
+      pose proof (sem_binary_operation_mse _ (penv_footprint_dec pe)).
+      transport H3. subst.
+      monadInv TRANSL. eauto.
+    - intros. monadInv TR. econstructor; eauto.
+      erewrite <- transl_expr_typeof; eauto. inv HP.
+      pose proof (sem_cast_mse _ (penv_footprint_dec pe)).
+      transport H1. subst. eauto.
+    - intros. monadInv TR.
+      replace (ClightP.genv_cenv ge) with (genv_cenv tge).
+      constructor. cbn. monadInv TRANSL. reflexivity.
+    - intros. monadInv TR.
+      replace (ClightP.genv_cenv ge) with (genv_cenv tge).
+      constructor. cbn. monadInv TRANSL. reflexivity.
+    - intros. specialize (H0 _ TR).
+      econstructor; eauto. cbn.
+      erewrite <- transl_expr_typeof; eauto.
+      inv HP. eapply deref_loc_mse; eauto. apply penv_footprint_dec.
+    - intros. monadInv TR. inv HP.
+      specialize (MDIFF _ _ H) as (b & A & B).
+      econstructor. eapply eval_Evar_global.
+      + edestruct (e ! id) eqn: X; eauto.
+        exfalso. eapply HE; eauto.
+      + eauto.
+      + inv B. eapply deref_loc_value; eauto.
+    - intros. monadInv TR. now constructor.
+    - intros. monadInv TR. apply eval_Evar_global; eauto.
+    - intros. monadInv TR. constructor. eauto.
+    - intros. monadInv TR. monadInv TRANSL. econstructor; eauto.
+      erewrite <- transl_expr_typeof; eauto.
+    - intros. monadInv TR. monadInv TRANSL.
+      eapply eval_Efield_union; eauto.
+      erewrite <- transl_expr_typeof; eauto.
+  Qed.
+
+  Lemma eval_expr_correct:
+    forall e le m tm pe,
+      ptree_disjoint e pe ->
+      penv_match se (pe, m) tm ->
+      forall expr v,
+          ClightP.eval_expr ge e le pe m expr v ->
+          forall texpr (TR: transl_expr expr = OK texpr),
+            Clight.eval_expr tge e le tm texpr (value_of v).
+  Proof. apply eval_expr_lvalue_correct. Qed.
+
+  Lemma eval_lvalue_correct:
+    forall e le m tm pe,
+      ptree_disjoint e pe ->
+      penv_match se (pe, m) tm ->
+      forall expr b ofs bf,
+        ClightP.eval_lvalue ge e le pe m expr b ofs bf ->
+        forall texpr (TR: transl_expr expr = OK texpr),
+          Clight.eval_lvalue tge e le tm texpr b ofs bf.
+  Proof. apply eval_expr_lvalue_correct. Qed.
+
+  Lemma eval_exprlist_correct:
+    forall e le m tm pe,
+      ptree_disjoint e pe ->
+      penv_match se (pe, m) tm ->
+      forall es tys vs,
+          ClightP.eval_exprlist ge e le pe m es tys vs ->
+          forall tes (TR: transl_exprlist es = OK tes),
+            Clight.eval_exprlist tge e le tm tes tys vs.
+  Proof.
+    intros until es. induction es.
+    - intros. monadInv TR. inv H1. constructor.
+    - intros * HEV * HTR.
+      monadInv HTR. inv HEV.
+      eapply eval_expr_correct in H3; eauto.
+      pose proof (sem_cast_mse _ (penv_footprint_dec pe)).
+      inv H0. transport H4. subst.
+      econstructor; eauto.
+      cbn. erewrite <- transl_expr_typeof; eauto.
+  Qed.
+
+  Hint Extern 1 (Transport _ _ _ _ _) =>
+         set_le_transport @assign_loc : typeclass_instances.
+
+  Lemma penv_footprint_in pe id pv b i:
+    pe ! id = Some pv ->
+    Genv.find_symbol se id = Some b ->
+    0 <= i < psizeof_ty (type_of pv) ->
+    locsp se (penv_footprint pe) b i.
+  Proof.
+    intros A B C. unfold locsp, penv_footprint.
+    apply Exists_exists. exists (id, psizeof pv). split.
+    - apply PTree.elements_correct in A.
+      apply in_map_iff. exists (id, pv). split; eauto.
+    - unfold locp. split; eauto.
+      destruct pv. unfold psizeof. apply C.
+  Qed.
+
+  (* Lemma pmatch_valid_access m b ofs v ch ty: *)
+  (*   pvalue_match b ofs v m -> *)
+  (*   Mem.valid_access ?m1 ?chunk ?b ?ofs Writable *)
+
+  Lemma footprint_same pe id ty old_v new_v:
+    pe ! id = Some (ClightP.Val old_v ty) ->
+    locsp se (penv_footprint (PTree.set id (ClightP.Val new_v ty) pe)) =
+      locsp se (penv_footprint pe).
+  Proof.
+    intros A.
+    apply Axioms.functional_extensionality. intros b.
+    apply Axioms.functional_extensionality. intros ofs.
+    apply PropExtensionality.propositional_extensionality; split; intros B.
+    - unfold locsp in *.
+      rewrite Exists_exists in *. destruct B as ([x y] & X & Y).
+      exists (x, y). split; eauto.
+      unfold penv_footprint in *.
+      rewrite in_map_iff in *.
+      destruct X as ([u v] & U & V). inv U.
+      eexists (x, (if peq x id then ClightP.Val old_v ty else v)).
+      apply PTree.elements_complete in V.
+      rewrite PTree.gsspec in V.
+      destruct peq; subst; split; inv V; eauto using PTree.elements_correct.
+    - unfold locsp in *.
+      rewrite Exists_exists in *. destruct B as ([x y] & X & Y).
+      exists (x, y). split; eauto.
+      unfold penv_footprint in *.
+      rewrite in_map_iff in *.
+      destruct X as ([u v] & U & V). inv U.
+      eexists (x, (if peq x id then ClightP.Val new_v ty else v)).
+      split.
+      + destruct peq. subst. apply PTree.elements_complete in V.
+        rewrite A in V. inv V. reflexivity. reflexivity.
+      + apply PTree.elements_correct.
+        rewrite PTree.gsspec.
+        destruct peq. subst. reflexivity.
+        apply PTree.elements_complete in V. assumption.
+  Qed.
+
+  Lemma functions_translated v fd:
+    Genv.find_funct (ClightP.genv_genv ge) v = Some fd ->
+    exists i tfd, Genv.find_funct tge v = Some tfd /\ transl_fundef i fd = OK tfd.
+  Admitted.
+
+  Lemma type_of_fundef_preserved id fd tfd:
+    transl_fundef id fd = OK tfd -> ClightP.type_of_fundef fd = type_of_fundef tfd.
+  Proof.
+    intros H. destruct fd.
+    - monadInv H. cbn. destruct f. monadInv EQ. cbn. reflexivity.
+    - monadInv H. reflexivity.
+  Qed.
+
+  Lemma external_call_match ef vargs pe m tm t vres m':
+    penv_match se (pe, m) tm ->
+    external_call ef (ClightP.genv_genv ge) vargs m t vres m' ->
+    exists tm', external_call ef tge vargs tm t vres tm' /\ penv_match se (pe, m') tm'.
+  Proof.
+  Admitted.
+
+  Lemma free_list_match pe m bs m' tm:
+    penv_match se (pe, m) tm -> Mem.free_list m bs = Some m' ->
+    exists tm', Mem.free_list tm bs = Some tm' /\ penv_match se (pe, m') tm'.
+  Proof.
+  Admitted.
+
+  Lemma pmatch_call_cont pe k kt:
+    pmatch_cont (k, pe) kt ->
+    pmatch_cont (ClightP.call_cont k, pe) (call_cont kt).
+  Proof.
+    intros H.
+    set (P := fun '(k, pe) kt => pmatch_cont (ClightP.call_cont k, pe) (call_cont kt)).
+    eapply pmatch_cont_ind with (P := P) in H; subst P; cbn; eauto.
+    constructor.
+    intros. constructor; eauto.
+  Qed.
+
+  Lemma pmatch_is_call_cont pe k kt:
+    pmatch_cont (k, pe) kt ->
+    ClightP.is_call_cont k ->
+    Clight.is_call_cont kt.
+  Proof. intros. inv H; auto. Qed.
+
+  Lemma blocks_of_env_same e:
+    ClightP.blocks_of_env ge e = blocks_of_env tge e.
+  Proof.
+    unfold ClightP.blocks_of_env, blocks_of_env.
+    f_equal.
+    unfold ClightP.block_of_binding, block_of_binding.
+    subst ge tge. monadInv TRANSL. cbn. reflexivity.
+  Qed.
+
+  Lemma transl_select_switch n sl tsl:
+    transl_lbl_stmt sl = OK tsl ->
+    transl_lbl_stmt (ClightP.select_switch n sl) = OK (select_switch n tsl).
+  Proof.
+  Admitted.
+
+  Lemma transl_seq_of_labeled_statement sl tsl:
+    transl_lbl_stmt sl = OK tsl ->
+    transl_statement (ClightP.seq_of_labeled_statement sl) = OK (seq_of_labeled_statement tsl).
+  Proof.
+  Admitted.
+
+  Lemma pmatch_function_entry1 pe m tm f tf vargs m' e le:
+    penv_match se (pe, m) tm ->
+    transl_function f = OK tf ->
+    ClightP.function_entry1 ge f vargs m e le m' ->
+    exists tm', function_entry1 tge tf vargs tm e le tm' /\
+             penv_match se (pe, m') tm' /\
+             ptree_disjoint e pe.
+  Proof.
+  Admitted.
+
+  Lemma pmatch_find_label pe s ts k tk s' k' lbl:
+    transl_statement s = OK ts ->
+    pmatch_cont (k, pe) tk ->
+    ClightP.find_label lbl s (ClightP.call_cont k) = Some (s', k') ->
+    exists ts' tk',
+      find_label lbl ts (call_cont tk) = Some (ts', tk') /\
+        transl_statement s' = OK ts' /\
+        pmatch_cont (k', pe) tk'.
+  Proof.
+  Admitted.
+
+  Lemma load_result_same ty ch v:
+    access_mode ty = By_value ch ->
+    Val.load_result (chunk_of_type (typ_of_type ty)) v =
+      Val.load_result ch v.
+  Admitted.
+
+  Lemma pmatch_cont_set_pe k tk pe id v v':
+    pe ! id = Some v ->
+    pmatch_cont (k, pe) tk ->
+    pmatch_cont (k, (PTree.set id v' pe)) tk.
+  Admitted.
+
+  Lemma step_correct:
+    forall s1 pe t s1' pe',
+      ClightP.step1 ge (s1, pe) t (s1', pe') ->
+      forall s2 : state,
+        pmatch_state se (s1, pe) s2 ->
+        exists s2' : state, Clight.step1 tge s2 t s2' /\ pmatch_state se (s1', pe') s2'.
+  Proof.
+    induction 1; intros S2 MS; inv MS.
+    (* assign *)
+    - monadInv TRS. pose proof H2 as HA.
+      eapply eval_lvalue_correct in H; eauto.
+      eapply eval_expr_correct in H0; eauto.
+      inv MP. clear pe. rename pe0 into pe.
+      pose proof (sem_cast_mse _ (penv_footprint_dec pe)).
+      transport H1. subst.
+      pose proof (assign_loc_mse _ (penv_footprint_dec pe)).
+      transport H2.
+      eexists. split.
+      + econstructor; eauto.
+        erewrite <- !transl_expr_typeof; eauto.
+        erewrite <- !transl_expr_typeof; eauto.
+        monadInv TRANSL. eauto.
+      + constructor; eauto.
+        constructor; eauto.
+        intros id pv Hpv. specialize (MDIFF _ _ Hpv) as (b & HB1 & HB2).
+        exists b. split; eauto.
+        eapply unchanged_on_pvalue_match; eauto.
+        instantiate (1 := locsp se (penv_footprint pe)).
+        * inv H5.
+          -- eapply Mem.store_unchanged_on; eauto.
+             intros i Hi contra.
+             eapply diff_perm; eauto.
+             inv HA.
+             ++ exploit Mem.store_valid_access_3; eauto. intros [A B].
+                assert (Mem.perm m loc i Cur Writable); eauto with mem.
+                apply A. replace chunk0 with chunk by congruence. eauto.
+             (* this case is legit when array is considered *)
+             ++ congruence.
+          -- eapply Mem.storebytes_unchanged_on; eauto.
+             intros i Hi contra.
+             eapply diff_perm; eauto.
+             inv HA.
+             ++ congruence.
+             ++ assert (Mem.perm m loc i Cur Writable); eauto with mem.
+                eapply Mem.storebytes_range_perm in H18. apply H18.
+                pose proof (loadbytes_mse _ (penv_footprint_dec pe)).
+                transport H17. subst. replace x1 with bytes by congruence.
+                eauto.
+          -- inv H2. eapply Mem.store_unchanged_on; eauto.
+             intros i Hi contra.
+             eapply diff_perm. apply MSAME. apply contra.
+             assert (Mem.perm m loc i Cur Writable).
+             2: { clear - H2. eauto with mem. }
+             inv HA. inv H17.
+             exploit Mem.store_valid_access_3. apply H25. intros [A B].
+             apply A. eauto.
+        * intros i Hi. eapply penv_footprint_in; eauto.
+    (* set *)
+    - monadInv TRS.
+      eapply eval_expr_correct in H; eauto.
+      eexists. split; constructor; eauto.
+    (* update *)
+    - monadInv TRS.
+      exploit eval_expr_type_same. apply H1. intros Hty.
+      eapply eval_expr_correct in H1; eauto.
+      inv MP. clear pe. rename pe0 into pe.
+      exploit MDIFF. apply H. intros (b & HB1 & HB2).
+      inv HB2. eapply Mem.valid_access_store in H10 as (m' & Hm').
+      eexists. split.
+      + econstructor.           (* assign *)
+        * eapply eval_Evar_global.
+          edestruct (e ! id) eqn: X.
+          exfalso. eapply DISJ; eauto. reflexivity.
+          apply HB1.
+        * eauto.
+        * cbn in *.
+          exploit transl_expr_typeof. apply EQ.
+          intros Hty2.
+          replace (typeof x) with ty by congruence.
+          apply cast_val_casted; eauto.
+        * eapply assign_loc_value; eauto.
+      + constructor; eauto.     (* match *)
+        * eapply pmatch_cont_set_pe; eauto.
+        * constructor.
+          -- erewrite footprint_same; eauto.
+             eapply mse_preserve; eauto.
+             intros i Hi. eapply penv_footprint_in; eauto.
+             cbn. erewrite <- size_type_chunk; eauto.
+          -- intros idx vx Hx.
+             destruct (peq id idx).
+             ++ subst. rewrite PTree.gss in Hx. inv Hx.
+                exists b. split; eauto. econstructor; eauto.
+                (* load same value *)
+                eapply Mem.load_store_same in Hm'.
+                exploit val_casted_has_type; eauto.
+                intros contra. subst. inv H0.
+                intros HTY.
+                rewrite Hm'. f_equal.
+                apply Val.load_result_same in HTY.
+                erewrite <- load_result_same; eauto.
+                (* valid_access *)
+                eapply Mem.store_valid_access_1; eauto.
+                eapply Mem.store_valid_access_3; eauto.
+             ++ rewrite PTree.gso in Hx; eauto.
+                exploit MDIFF. apply Hx.
+                intros (bx & BX1 & BX2). exists bx. split; auto.
+                assert (b <> bx).
+                {
+                  intros contra. subst.
+                  apply n. eapply Genv.find_symbol_injective; eauto.
+                }
+                eapply unchanged_on_pvalue_match; eauto.
+                eapply Mem.store_unchanged_on. apply Hm'.
+                instantiate (1 := fun bi _ => bi = bx).
+                intuition. intuition.
+        * intros idx [bx ofsx] vx HE HPE.
+          destruct (peq idx id). subst.
+          -- rewrite PTree.gss in HPE. inv HPE.
+             eapply DISJ; eauto.
+          -- rewrite PTree.gso in HPE; eauto.
+
+    (* call *)
+    - monadInv TRS. clear pe. rename pe0 into pe.
+      eapply eval_expr_correct in H0; eauto.
+      eapply eval_exprlist_correct in H1; eauto.
+      exploit functions_translated. eauto. intros (i & tfd & HFD1 & HFD2).
+      eexists. split.
+      + econstructor; eauto.
+        erewrite <- transl_expr_typeof; eauto.
+        cbn. unfold ClightP.genv_genv in *. cbn in H2.
+        exploit type_of_fundef_preserved. eauto. intros <-. eauto.
+      + constructor; eauto.
+        constructor; eauto.
+
+    (* builtin *)
+    - monadInv TRS.
+      eapply eval_exprlist_correct in H; eauto.
+      exploit external_call_match; eauto. intros (mt' & HEC & HM).
+      eexists. split.
+      + econstructor; eauto.
+      + constructor; eauto.
+
+    (* sequence *)
+    - monadInv TRS.
+      eexists. split; repeat (constructor; eauto).
+
+    (* skip sequence *)
+    - monadInv TRS. inv MK.
+      eexists. split. constructor. constructor; eauto.
+
+    (* continue sequence *)
+    - monadInv TRS. inv MK.
+      eexists. split. constructor. constructor; eauto.
+
+    (* break sequence *)
+    - monadInv TRS. inv MK.
+      eexists. split. constructor. constructor; eauto.
+
+    (* ifthenelse *)
+    - monadInv TRS. clear pe. rename pe0 into pe.
+      inv MP.
+      pose proof (bool_val_mse _ (penv_footprint_dec pe)).
+      transport H0. subst.
+      eapply eval_expr_correct in H; eauto.
+      eexists. split. econstructor; eauto.
+      cbn. erewrite <- transl_expr_typeof; eauto.
+      constructor; eauto. destruct x2; eauto.
+      all: constructor; eauto.
+
+    (* loop *)
+    - monadInv TRS. eexists. split.
+      constructor. repeat (constructor; eauto).
+
+    (* skip-or-continue loop *)
+    - inv MK. destruct H; subst; monadInv TRS;
+        eexists; split; repeat (constructor; eauto).
+
+    (* break loop1 *)
+    - monadInv TRS. inv MK. eexists; split.
+      eapply step_break_loop1.
+      constructor; eauto.
+
+    (* skip loop2 *)
+    - monadInv TRS. inv MK. eexists; split.
+      constructor. constructor; eauto.
+      cbn. rewrite H4. cbn. rewrite H5. reflexivity.
+
+    (* break loop2 *)
+    - monadInv TRS. inv MK. eexists; split.
+      constructor. constructor; eauto.
+
+    (* return None *)
+    - monadInv TRS.
+      exploit free_list_match; eauto. intros (tm' & HFL & HM).
+      eexists; split.
+      constructor. rewrite <- blocks_of_env_same; eauto.
+      constructor; eauto.
+      apply pmatch_call_cont. auto.
+
+    (* return Some *)
+    - monadInv TRS.
+      exploit eval_expr_correct; eauto. intros HEV.
+      exploit free_list_match; eauto. intros (tm' & HFL & HM).
+      inv MP. clear pe. rename pe0 into pe.
+      pose proof (sem_cast_mse _ (penv_footprint_dec pe)).
+      transport H0. subst.
+      eexists. split.
+      econstructor; eauto.
+      erewrite <- transl_expr_typeof; eauto.
+      monadInv TRF. apply H3.
+      rewrite <- blocks_of_env_same. apply HFL.
+      constructor; eauto.
+      apply pmatch_call_cont. eauto.
+
+    (* skip call *)
+    - monadInv TRS.
+      exploit free_list_match; eauto. intros (tm' & HFL & HM).
+      eexists. split.
+      constructor. eapply pmatch_is_call_cont; eauto.
+      rewrite <- blocks_of_env_same. eauto.
+      constructor; eauto.
+
+    (* switch *)
+    - monadInv TRS.
+      eapply eval_expr_correct in H; eauto. cbn in *.
+      eexists; split.
+      econstructor; eauto.
+      erewrite <- transl_expr_typeof; eauto.
+      constructor; eauto.
+      apply transl_seq_of_labeled_statement. apply transl_select_switch. eauto.
+      constructor. eauto.
+
+    (* skip-break switch *)
+    - inv MK. destruct H; subst;
+        monadInv TRS; eexists; split; constructor; eauto.
+
+    (* continue switch *)
+    - monadInv TRS. inv MK. eexists. split.
+      eapply step_continue_switch.
+      constructor; eauto.
+
+    (* label *)
+    - monadInv TRS. eexists; split; constructor; eauto.
+
+    (* goto *)
+    - monadInv TRS. pose proof TRF. monadInv TRF.
+      exploit pmatch_find_label; eauto.
+      intros (ts' & tk' & HLB & HS & HK).
+      eexists; split.
+      constructor; eauto.
+      constructor; eauto.
+
+    (* internal function *)
+    - exploit functions_translated; eauto. intros (i & tfd & HFD & HTF).
+      monadInv HTF.
+      exploit pmatch_function_entry1; eauto. intros (tm' & HFE & HM & HE).
+      eexists. split.
+      constructor; eauto.
+      constructor; eauto.
+      monadInv EQ. cbn. eauto.
+
+    (* external function *)
+    - exploit functions_translated; eauto. intros (i & tfd & HFD & HTF).
+      monadInv HTF.
+      exploit external_call_match; eauto. intros (tm' & HEC & HM).
+      eexists. split.
+      econstructor; eauto.
+      constructor; eauto.
+
+    (* return *)
+    - inv MK.
+      eexists. split. constructor. constructor; eauto.
+  Qed.
+
+End PRESERVATION.
+
+Theorem transl_program_correct prog tprog:
+  transl_program prog = OK tprog ->
+  forward_simulation cc_id cc_penv (ClightP.clightp1 prog) (Clight.semantics1 tprog).
+Proof.
+  intros H. constructor. econstructor.
+  - admit.
+  - admit.
+  - intros se1 se2 wb Hse Hse1. instantiate (1 := fun _ _ _ => _). cbn beta.
+    eapply forward_simulation_step with (match_states := pmatch_state se2).
+    + admit.
+    + admit.
+    + admit.
+    + cbn.
+      intros. destruct s1, s1'.
+      eapply step_correct; eauto.
+      inv Hse. eauto.
+Admitted.
+
+
+(*
 Section ClightM.
 
   Variable ge: Clight.genv.
@@ -1065,3 +2207,4 @@ Program Definition eclight2 (p: program) :=
                          (fun _ => final_state)
                          globalenv p
   |}.
+*)
